Improve performance of register allocation.

Coherence/AllocationAlgo.v
@@ -1,31 +1,17 @@
 Require Import CSet Le Arith.Compare_dec.
 
-Require Import Plus Util Map Status.
+Require Import Plus Util Map CMap Status.
 Require Import Val Var Env EnvTy IL Annotation Liveness Fresh Sim MoreList.
 Require Import Coherence Allocation.
 
 Set Implicit Arguments.
 
-Section ParametricDualFold.
-  Variables A X Y : Type.
-  Hypothesis f : A -> X -> Y -> status A : Type.
 
-  Fixpoint dfold (a:A) (L:list X) (L':list Y) : status A :=
-    match L, L' with
-      | x::L, y::L' => sdo a' <- f a x y;
-                      dfold a' L L'
-      | nil, nil => Success a
-      | _, _ => Error "dfold: argument list size mismatch"
-    end.
-End ParametricDualFold.
-
-Arguments dfold [A] [X] [Y] f a L L'.
-
-Fixpoint linear_scan (st:stmt) (an: ann (set var)) (ϱ:var -> var)
-  : status (var -> var) :=
+Fixpoint linear_scan (st:stmt) (an: ann (set var)) (ϱ:Map [var, var])
+  : status (Map [var, var]) :=
  match st, an with
     | stmtExp x e s, ann1 lv ans =>
-      let xv := least_fresh (lookup_set ϱ (getAnn ans\{{x}})) in
+      let xv := least_fresh (SetConstructs.map (findt ϱ 0) (getAnn ans\{{x}})) in
         linear_scan s ans (ϱ[x<- xv])
     | stmtIf _ s t, ann2 lv ans ant =>
       sdo ϱ' <- linear_scan s ans ϱ;
@@ -33,29 +19,28 @@ Fixpoint linear_scan (st:stmt) (an: ann (set var)) (ϱ:var -> var)
     | stmtGoto _ _, ann0 _ => Success ϱ
     | stmtReturn _, ann0 _ => Success ϱ
     | stmtExtern x f Y s, ann1 lv ans =>
-      let xv := least_fresh (lookup_set ϱ (getAnn ans\{{x}})) in
+      let xv := least_fresh (SetConstructs.map (findt ϱ 0) (getAnn ans\{{x}})) in
       linear_scan s ans (ϱ[x<- xv])
     | stmtLet Z s t, ann2 _ ans ant =>
-      let Z' := fresh_list least_fresh (lookup_set ϱ (getAnn ans\of_list Z)) (length Z) in
+      let Z' := fresh_list least_fresh (SetConstructs.map (findt ϱ 0) (getAnn ans\of_list Z)) (length Z) in
       sdo ϱ' <- linear_scan s ans (ϱ[Z <-- Z']);
         linear_scan t ant ϱ'
     | _, _ => Error "linear_scan: Annotation mismatch"
   end.
 
-
-Hint Extern 10 (agree_on _ _?a ?a) => reflexivity.
-
 Lemma linear_scan_ssa_agree' i s al ϱ ϱ' LV alv G
       (sd:ssa s al)
       (LS:live_sound i LV s alv)
       (allocOK:linear_scan s alv ϱ = Success ϱ')
-: agree_on eq (G \ (snd (getAnn al) \ fst (getAnn al))) ϱ ϱ'.
+: agree_on eq (G \ (snd (getAnn al) \ fst (getAnn al))) (findt ϱ 0) (findt ϱ' 0).
 Proof.
   general induction LS; inv sd; simpl in * |- *; try monadS_inv allocOK; eauto.
   - exploit IHLS; eauto.
+    rewrite <- map_update_update_agree in X.
     rewrite H8 in X; simpl in *.
     eapply agree_on_incl.
-    eapply agree_on_update_inv. eapply X.
+    eapply agree_on_update_inv.
+    eapply X.
     instantiate (1:=G).
     pose proof (ssa_incl H7); eauto. rewrite H8 in H1. simpl in *.
     revert H4 H1; clear_all; cset_tac; intuition.
@@ -67,6 +52,7 @@ Proof.
     instantiate (1:=G). rewrite <- H7. clear_all; intro; cset_tac; intuition.
     instantiate (1:=G). rewrite <- H7. clear_all; intro; cset_tac; intuition.
   - exploit IHLS; eauto.
+    rewrite <- map_update_update_agree in X.
     rewrite H9 in X; simpl in *.
     eapply agree_on_incl.
     eapply agree_on_update_inv. eapply X.
@@ -76,6 +62,7 @@ Proof.
     invc H. specialize (H1 a). cset_tac; intuition.
   - exploit IHLS1; eauto.
     exploit IHLS2; eauto.
+    rewrite <- map_update_list_update_agree in X.
     rewrite H9 in X. rewrite H12 in X0. simpl in *.
     etransitivity; try eapply X0.
     eapply agree_on_incl. eapply update_with_list_agree_inv; try eapply X; eauto.
@@ -86,37 +73,20 @@ Proof.
     specialize (H2 a). specialize (H3 a). cset_tac; intuition.
     eapply agree_on_incl; eauto. instantiate (1:=G).
     rewrite <- H7. clear_all; cset_tac; intuition; eauto.
+    rewrite fresh_list_length; eauto.
 Qed.
 
 Lemma linear_scan_ssa_agree i s al ϱ ϱ' LV alv
       (sd:ssa s al)
       (LS:live_sound i LV s alv)
       (allocOK:linear_scan s alv ϱ = Success ϱ')
-: agree_on eq (fst (getAnn al)) ϱ ϱ'.
+: agree_on eq (fst (getAnn al)) (findt ϱ 0) (findt ϱ' 0).
 Proof.
-  general induction LS; inv sd; simpl in * |- *; try monadS_inv allocOK; eauto.
-  - exploit IHLS; eauto.
-    rewrite H8 in X; simpl in *.
-    eapply agree_on_incl.
-    eapply agree_on_update_inv; eauto. cset_tac; intuition.
-  - exploit IHLS1; eauto.
-    exploit IHLS2; eauto.
-    rewrite H11 in X. rewrite H12 in X0. simpl in *.
-    etransitivity; eauto.
-  - exploit IHLS; eauto.
-    rewrite H9 in X; simpl in *.
-    eapply agree_on_incl.
-    eapply agree_on_update_inv; eauto. cset_tac; intuition.
-  - exploit IHLS1; eauto.
-    exploit IHLS2; eauto.
-    rewrite H9 in X. rewrite H12 in X0. simpl in *.
-    etransitivity; try eapply X0.
-    eapply agree_on_incl. eapply update_with_list_agree_inv; try eapply X; eauto.
-    rewrite fresh_list_length; eauto.
-    revert H5; clear_all; cset_tac; intuition; eauto.
+  eapply agree_on_incl.
+  eapply linear_scan_ssa_agree'; eauto.
+  instantiate (1:=fst (getAnn al)).
+  cset_tac; intuition.
 Qed.
-
-Hint Extern 10 (Subset ?a (_ ∪ ?a)) => eapply incl_right.
 
 Lemma locally_inj_live_agree s ϱ ϱ' ara alv LV
       (LS:live_sound Functional LV s alv)
@@ -200,19 +170,20 @@ Proof.
       decide (a ∈ of_list Z); eauto.
 Qed.
 
-Lemma linear_scan_correct (ϱ:var->var) LV s alv ϱ' al
+Lemma linear_scan_correct (ϱ:Map [var,var]) LV s alv ϱ' al
       (LS:live_sound Functional LV s alv)
-      (inj:injective_on (getAnn alv) ϱ)
+      (inj:injective_on (getAnn alv) (findt ϱ 0))
       (allocOK:linear_scan s alv ϱ = Success ϱ')
       (incl:getAnn alv ⊆ fst (getAnn al))
       (sd:ssa s al)
-: locally_inj ϱ' s alv.
+: locally_inj (findt ϱ' 0) s alv.
 Proof.
   intros.
   general induction LS; simpl in *; try monadS_inv allocOK; invt ssa;
     eauto 10 using locally_inj, injective_on_incl.
   - exploit IHLS; try eapply allocOK; eauto.
-    + eapply injective_on_incl.
+    + eapply injective_on_agree; [| eapply map_update_update_agree].
+      eapply injective_on_incl.
       eapply injective_on_fresh; eauto using injective_on_incl, least_fresh_spec.
       eauto.
     + rewrite H8. simpl in *. rewrite <- incl.
@@ -224,7 +195,9 @@ Proof.
       econstructor. eauto using injective_on_incl.
       eapply injective_on_agree; try eapply inj.
       eapply agree_on_incl.
-      eapply agree_on_update_inv. eapply X0.
+      eapply agree_on_update_inv.
+      etransitivity. eapply map_update_update_agree.
+      eapply X0.
       revert H4 incl; clear_all; cset_tac; intuition. invc H0. eauto.
       exploit locally_injective; eauto.
       eapply injective_on_agree; try eapply X0.
@@ -234,6 +207,7 @@ Proof.
       decide (x === a). intuition.
       left. eapply H0; eauto. cset_tac; intuition.
       eapply injective_on_incl.
+      eapply injective_on_agree; [| eapply map_update_update_agree].
       eapply injective_on_fresh; eauto.
       Focus 2.
       eapply least_fresh_spec.
@@ -250,7 +224,7 @@ Proof.
     eapply injective_on_agree; eauto using agree_on_incl.
     rewrite H12; simpl. rewrite <- incl; eauto.
     econstructor; eauto.
-    assert (agree_on eq D ϱ ϱ'). etransitivity; eauto.
+    assert (agree_on eq D (findt ϱ 0) (findt ϱ' 0)). etransitivity; eauto.
     eapply injective_on_agree; eauto. eauto using agree_on_incl.
     eapply locally_inj_live_agree. eauto. eauto. eauto.
     rewrite H11; simpl; eauto.
@@ -261,6 +235,7 @@ Proof.
     rewrite H11; simpl. rewrite <- incl; eauto.
   - exploit IHLS; try eapply allocOK; eauto.
     + eapply injective_on_incl.
+      eapply injective_on_agree; [| eapply map_update_update_agree].
       eapply injective_on_fresh; eauto using injective_on_incl, least_fresh_spec.
       eauto.
     + rewrite H9. simpl in *. rewrite <- incl.
@@ -272,7 +247,9 @@ Proof.
       econstructor. eauto using injective_on_incl.
       eapply injective_on_agree; try eapply inj.
       eapply agree_on_incl.
-      eapply agree_on_update_inv. eapply X0.
+      eapply agree_on_update_inv.
+      etransitivity. eapply map_update_update_agree.
+      eapply X0.
       revert H5 incl; clear_all; cset_tac; intuition. invc H0. eauto.
       exploit locally_injective; eauto.
       eapply injective_on_agree; try eapply X0.
@@ -282,6 +259,7 @@ Proof.
       decide (x === a). intuition.
       left. eapply H0; eauto. cset_tac; intuition.
       eapply injective_on_incl.
+      eapply injective_on_agree; [| eapply map_update_update_agree].
       eapply injective_on_fresh; eauto.
       Focus 2.
       eapply least_fresh_spec.
@@ -290,8 +268,10 @@ Proof.
   - simpl in *.
     exploit linear_scan_ssa_agree; try eapply EQ; simpl; eauto using live_sound.
     exploit linear_scan_ssa_agree; try eapply EQ0; simpl; eauto using live_sound.
+    rewrite <- map_update_list_update_agree in X.
     exploit IHLS1; eauto.
-    + eapply injective_on_incl.
+    + eapply injective_on_agree; [| eapply map_update_list_update_agree].
+      eapply injective_on_incl.
       instantiate (1:=getAnn als \ of_list Z ++ of_list Z).
       eapply injective_on_fresh_list; eauto.
       eapply injective_on_incl; eauto.
@@ -300,11 +280,12 @@ Proof.
       eapply fresh_list_unique, least_fresh_spec.
       clear_all; cset_tac; intuition.
       decide (a ∈ of_list Z); intuition.
+      rewrite fresh_list_length; eauto.
     + rewrite H9. simpl. rewrite <- incl.
       revert H0; clear_all; cset_tac; intuition.
       specialize (H0 a). cset_tac; intuition.
       decide (a ∈ of_list Z); intuition.
-    + assert (injective_on lv ϱ').
+    + assert (injective_on lv (findt ϱ' 0)).
       eapply injective_on_incl.
       eapply injective_on_agree; try eapply inj; eauto.
       etransitivity.
@@ -336,9 +317,11 @@ Proof.
         specialize (H0 a). cset_tac; intuition.
         decide (a ∈ of_list Z); intuition.
         eapply injective_on_incl. instantiate (1:=(getAnn als \ of_list Z) ∪ of_list Z).
-        eapply injective_on_agree with (ϱ:=(ϱ [Z <--
-         fresh_list least_fresh (lookup_set ϱ (getAnn als \ of_list Z))
-           (length Z)])).
+        eapply injective_on_agree with
+        (ϱ:=MapUpdate.update_with_list Z
+                             (fresh_list least_fresh
+                                         (SetConstructs.map (findt ϱ 0) (getAnn als \ of_list Z))
+                                         (length Z)) (findt ϱ 0)).
         eapply injective_on_fresh_list; eauto using injective_on_incl.
         rewrite fresh_list_length; eauto.
         eapply fresh_list_spec. eapply least_fresh_spec.
@@ -353,6 +336,7 @@ Proof.
         revert X3 H6; clear_all; cset_tac; intuition.
         specialize (X3 a); specialize (H6 a); cset_tac; intuition.
         clear_all; cset_tac; intuition. decide (a ∈ of_list Z); eauto.
+    + rewrite fresh_list_length; eauto.
 Qed.
 
 
