Fresh.v
@@ -1,27 +1,9 @@
 Require Import CSet Le Arith.Compare_dec.
 
 Require Import Plus Util Map.
-Require Import Env EnvTy IL InjectiveMapping.
+Require Import Env EnvTy IL.
 
 Set Implicit Arguments.
-
-Instance le_comp (a b: nat) : Computable (a < b).
-eapply lt_dec.
-Defined.
-
-(*Definition max a b := if [ a < b ] then b else a.
-Definition min a b := if [ a < b ] then a else b.*)
-
-Section PolyIter.
-  Variable A : Type.
-
-  Fixpoint iter n (s:A) (f: nat -> A-> A) :=
-    match n with
-        | 0 => s
-        | S n => iter n (f n s) f
-    end.
-
-End PolyIter.
 
 Definition fresh (s : set var) : var :=
   S(fold max s 0).
@@ -136,39 +118,6 @@ Section FreshList.
   Qed.
 End FreshList.
 
-Definition notincl {X} `{OrderedType X} (s t: set X) := forall x, x ∈ s -> x ∉ t.
-
-Lemma inverse_on_update_fresh (D:set var) (Z Z':list var) (ϱ ϱ' : var -> var)
- : inverse_on (D \ of_list Z) ϱ ϱ'
-  -> unique Z'
-  -> length Z = length Z'
-  -> notincl (of_list Z') (lookup_set ϱ (D \ of_list Z))
-  -> inverse_on D (update_with_list Z Z' ϱ)
-                 (update_with_list Z' Z ϱ').
-Proof.
-  intros. eapply length_length_eq in H1.
-  hnf; intros. lud. decide(x ∈ of_list Z).
-  general induction H1; simpl in *; eauto; dcr. cset_tac; exfalso; eauto.
-  lud. eapply add_iff in i. destruct i; eauto.
-  assert (y ∈ of_list YL). rewrite e.
-  eapply update_with_list_lookup_in; eauto using length_eq_length.
-  exfalso. eapply (@fresh_of_list _ _ YL y H4 H9).
-  exfalso; eauto.
-  eapply add_iff in i; destruct i; isabsurd.
-  eapply IHlength_eq; try eassumption.
-  hnf; intros. exfalso; cset_tac; eauto.
-  hnf; intros. intro. eapply lookup_set_spec in H11.
-  destruct H11; cset_tac; eauto. intuition.
-
-  erewrite update_with_list_no_update; eauto.
-  erewrite update_with_list_no_update; eauto.
-  eapply H; eauto. cset_tac ; eauto.
-  erewrite update_with_list_no_update; eauto. intro.
-  eapply H2; eauto.
-  eapply lookup_set_spec; cset_tac; intuition.
-  eexists x; eauto.
-Qed.
-
 Lemma inverse_on_update_fresh_list (D:set var) (Z:list var) (ϱ ϱ' : var -> var)
  : inverse_on (D \ of_list Z) ϱ ϱ'
   -> inverse_on D (update_with_list Z (fresh_list fresh (lookup_set ϱ (D \ of_list Z)) (length Z)) ϱ)
@@ -180,85 +129,6 @@ Proof.
   hnf; intros. intro. eapply (not_in_empty x).
   eapply fresh_list_spec; eauto using fresh_spec. cset_tac; eauto.
 Qed.
-
-Hint Extern 20 (Subset (?a \ _) ?a) => eapply minus_incl.
-Hint Extern 20 (Subset (?a \ _) ?a') => (is_evar a ; fail 1)
-                                        || (has_evar a ; fail 1)
-                                        || (is_evar a' ; fail 1)
-                                        || (has_evar a'; fail 1)
-                                        || eapply minus_incl.
-Hint Extern 20 => match goal with
-                   | [ H: ?a /\ ?b |- ?b ] => eapply H
-                   | [ H: ?a /\ ?b |- ?a ] => eapply H
-                 end.
-
-Section MapUpdate.
-  Open Scope fmap_scope.
-  Variable X : Type.
-  Context `{OrderedType X}.
-  Variable Y : Type.
-
-  Lemma update_unique_commute `{OrderedType Y} (XL:list X) (VL:list Y) E D x y
-  : length XL = length VL
-    -> unique (x::XL)
-    -> agree_on _eq D (E [x <- y] [XL <-- VL]) (E [XL <-- VL] [x <- y]).
-  Proof.
-    intros. eapply length_length_eq in H1.
-    general induction H1; simpl. reflexivity.
-    hnf; intros. lud. hnf in H2; simpl in *.
-    dcr. exfalso. eapply H8. econstructor. eapply H5.
-    exploit (IHlength_eq H _ E {x1} x0 y0). simpl in *; intuition.
-    hnf; intros. eapply H9. econstructor 2; eauto.
-    exploit X0. cset_tac; reflexivity. rewrite X1. lud.
-    exploit (IHlength_eq H _ E {x1} x0 y0). simpl in *; intuition.
-    hnf; intros. eapply H8. econstructor 2; eauto.
-    exploit X0. cset_tac; reflexivity. rewrite X1. lud.
-  Qed.
-
-  Lemma injective_on_agree `{OrderedType Y} D (ϱ ϱ': X -> Y)
-  : injective_on D ϱ
-    -> agree_on _eq D ϱ ϱ'
-    -> injective_on D ϱ'.
-  Proof.
-    intros. hnf; intros. eapply H1; eauto.
-    exploit H2; eauto. rewrite X0.
-    exploit H2; try eapply H3. rewrite X1. eauto.
-  Qed.
-
-End MapUpdate.
-
-Lemma injective_on_fresh_list X `{OrderedType X} Y `{OrderedType Y} XL YL (ϱ: X -> Y) `{Proper _ (_eq ==> _eq) ϱ} lv
-: injective_on lv ϱ
-  -> length XL = length YL
-  -> (of_list YL) ∩ (lookup_set ϱ lv) [=] ∅
-  -> unique XL
-  -> unique YL
-  -> injective_on (lv ∪ of_list XL) (ϱ [XL <-- YL]).
-Proof.
-  intros. eapply length_length_eq in H3.
-  general induction H3; simpl in * |- * ; eauto.
-  - eapply injective_on_incl; eauto. cset_tac; intuition.
-  - eapply injective_on_agree.
-    assert (lv ∪ { x; of_list XL} [=] {{x}} ∪ lv ∪ of_list XL) by (cset_tac; intuition; eauto).
-    rewrite H7. eapply IHlength_eq; auto.
-    Focus 2.
-    eapply injective_on_fresh. instantiate (1:=ϱ); eauto.
-    eapply injective_on_incl; eauto. instantiate (1:=y).
-    intro. eapply lookup_set_spec in H8. dcr.
-    eapply (not_in_empty (ϱ x0)). rewrite <- H4. cset_tac; intuition.
-    eapply lookup_set_spec; eauto. eapply H1.
-    hnf; intros. lud; eauto; try now exfalso; eauto.
-    dcr. cset_tac; intuition.
-    eapply lookup_set_spec in H12; dcr. lud.
-    eapply H8. rewrite <- H14; eauto. eapply InA_in; eauto.
-    cset_tac; intuition.
-    eapply H4. split. right; eauto.
-    eapply lookup_set_spec. eauto. eexists; eauto.
-    hnf; intros. lud; eauto; try now exfalso; eauto.
-    eapply update_unique_commute; eauto using length_eq_length.
-Qed.
-
-
 
 (*
 *** Local Variables: ***
